aarch64 crefine: consolidate machine op assumptions
Pull in all the sorried ccorres lemmas about missing machine op
assumptions into Machine_C as assumptions.

Add missing cache operations to Machine_C assumptions. On ARM and
ARM_HYP, these go a bit deeper, but unless we're modelling caches, all
we'd be showing is that a spec we copied from the C does the same thing
as the C, so for AARCH64 we are leaving the abstraction a bit higher,
resulting in these cache machine ops having ccorres assumptions:
- cleanCacheRange_RAM
- cleanCacheRange_PoU
- cleanInvalidateCacheRange_RAM
- invalidateCacheRange_I
- cleanByVA_PoU

Clear sorries related to clearMemory spec now that it's updated to match
the C.

Signed-off-by: Rafal Kolanski <rafal.kolanski@proofcraft.systems>

proof/crefine/AARCH64/Wellformed_C.thy
@@ -598,6 +598,11 @@ abbreviation(input)
 where
   "prioInvalid == seL4_InvalidPrio"
 
+(* caches *)
+
+definition cacheLineSize :: nat where
+  "cacheLineSize \<equiv> 6"
+
 (* generic lemmas with arch-specific consequences *)
 
 schematic_goal size_gpRegisters:
